-

math/Algorithm/Search.lean
@@ -1,20 +1,65 @@
 
+open Classical
+
 def find(nums: Array Nat)(target: Nat) : Option (Fin nums.size) := Id.run do
   for a in Array.finRange nums.size do
     if nums[a] = target then
       return a
   none
 
+structure FindResult (nums: Array Nat)(target: Nat) where
+  index : Fin nums.size
+  proof : nums[index] = target
+
+def findWithProof(nums: Array Nat)(target: Nat) : Option (FindResult nums target) := Id.run do
+  for a in Array.finRange nums.size do
+    if h: nums[a] = target then
+      return some ⟨a, h⟩
+  none
+
 theorem find_result_is_answer (nums: Array Nat)(target: Nat) :
-   ∀ a: Fin nums.size, find nums target = some a → nums[a] = target :=
-  by
+   ∀ a, find nums target = some a → nums[a] = target := by
     intro a
-    simp [find, ←Array.forIn_toList, List.forIn_cons]
+    intro h1
+    let f := fun x: FindResult nums target => Option.some x.index
+    have h: find nums target = (findWithProof nums target).bind f := by
+      simp [find, findWithProof, Id.run, Option.bind, f]
+      repeat rw [← Array.forIn_toList]
+      simp only [forIn, forIn', List.forIn', List.forIn'.loop]
+      generalize (Array.finRange nums.size).toList = list
+      induction list with
+      | nil =>
+        simp [List.forIn'.loop]
+      | cons a as ih =>
+        simp [List.forIn'.loop]
+        by_cases h3: nums[↑a] = target
+        . simp_all only [Fin.getElem_fin, ite_true, dite_true, f]
+        . sorry -- don't know how to do this yet
+    rw [h] at h1
+    simp [Option.bind]
+    cases ih: findWithProof nums target with
+    | none =>
+      have h2: (match findWithProof nums target, f with
+        | none, x => none
+        | some a, f => f a) = none := by
+        simp [ih]
+      simp_all
+    | some x =>
+      have h3: f x = some a := by
+        simp_all
+      have h4: x.index = a := by
+        rw [ih] at h1
+        simp [f] at h1
+        exact h1
+      have h5 := x.proof
+      simp [h4] at h5
+      exact h5
 
 
 
-
-
+-- 值得参考的实现：
+#check List.find?_eq_some_iff_append
+#check List.forIn'_cons
 
 
 example (nums: Array Nat)(target: Nat) : find nums target = none ↔ ∀ a: Fin nums.size, nums[a] ≠ target :=
